AwsCryptographicMaterialProviders/dafny/AwsCryptographyKeyStore/src/KMSKeystoreOperations.dfy
@@ -4,6 +4,9 @@ include "../Model/AwsCryptographyKeyStoreTypes.dfy"
 include "Structure.dfy"
 include "../../AwsCryptographicMaterialProviders/src/AwsArnParsing.dfy"
 include "../../AwsCryptographicMaterialProviders/src/Keyrings/AwsKms/AwsKmsMrkMatchForDecrypt.dfy"
+include "../../../dafny/AwsCryptographicMaterialProviders/src/AwsArnParsing.dfy"
+include "KmsArn.dfy"
+
 module {:options "/functionSyntax:4" } KMSKeystoreOperations {
   import opened Wrappers
   import opened UInt = StandardLibrary.UInt
@@ -15,21 +18,75 @@ module {:options "/functionSyntax:4" } KMSKeystoreOperations {
   import Structure
   import opened AwsArnParsing
   import AwsKmsMrkMatchForDecrypt
+  import KmsArn
+
+  function replaceRegion(arn : KMS.KeyIdType, region : KMS.RegionType) : KMS.KeyIdType
+  {
+    var parsed := ParseAwsKmsArn(arn);
+    if parsed.Failure? then
+      arn
+    else if !IsMultiRegionAwsKmsArn(parsed.value) then
+      arn
+    else
+      var newArn := parsed.value.ToArnString(Some(region));
+      if KMS.IsValid_KeyIdType(newArn) then
+        newArn
+      else
+        arn
+  }
+
+  function GetArn(kmsConfiguration: Types.KMSConfiguration, discoverdArn : KMS.KeyIdType) : KMS.KeyIdType
+  {
+    match kmsConfiguration {
+      case kmsKeyArn(arn) => arn
+      case kmsMRKeyArn(arn) => arn
+      case discovery(obj) =>  discoverdArn
+      case mrDiscovery(region) =>  replaceRegion(discoverdArn, region.region)
+    }
+  }
 
   predicate AttemptKmsOperation?(kmsConfiguration: Types.KMSConfiguration, encryptionContext: Structure.BranchKeyContext)
+    ensures AttemptKmsOperation?(kmsConfiguration, encryptionContext) && HasKeyId(kmsConfiguration)
+            ==> Compatible?(kmsConfiguration, encryptionContext[Structure.KMS_FIELD])
   {
     match kmsConfiguration
-    case kmsKeyArn(arn) => arn == encryptionContext[Structure.KMS_FIELD]
-    case kmsMRKeyArn(arn) =>
-      var ecArn := ParseAwsKmsArn(encryptionContext[Structure.KMS_FIELD]);
-      var kmsArn := ParseAwsKmsArn(arn);
-      if ecArn.Failure? || kmsArn.Failure? then
-        false
-      else
-        AwsKmsMrkMatchForDecrypt.AwsKmsMrkMatchForDecrypt(AwsKmsArnIdentifier(kmsArn.value), AwsKmsArnIdentifier(ecArn.value))
+    case kmsKeyArn(arn) => (arn == encryptionContext[Structure.KMS_FIELD]) && KmsArn.ValidKmsArn?(arn)
+    case kmsMRKeyArn(arn) => MrkMatch(arn, encryptionContext[Structure.KMS_FIELD]) && KmsArn.ValidKmsArn?(arn)
+    case discovery(obj) => KmsArn.ValidKmsArn?(encryptionContext[Structure.KMS_FIELD])
+    case mrDiscovery(obj) => KmsArn.ValidKmsArn?(encryptionContext[Structure.KMS_FIELD])
+  }
+
+  predicate Compatible?(kmsConfiguration: Types.KMSConfiguration, keyId : string)
+    requires(HasKeyId(kmsConfiguration))
+  {
+    match kmsConfiguration
+    case kmsKeyArn(arn) => (arn == keyId)
+    case kmsMRKeyArn(arn) => MrkMatch(arn, keyId)
+  }
+
+  predicate OptCompatible?(kmsConfiguration: Types.KMSConfiguration, keyId : Option<string>)
+    requires(HasKeyId(kmsConfiguration))
+  {
+    keyId.Some? && Compatible?(kmsConfiguration, keyId.value)
+  }
+
+  predicate MrkMatch(x : string, y : string)
+  {
+    var xArn := ParseAwsKmsArn(x);
+    var yArn := ParseAwsKmsArn(y);
+    if xArn.Failure? || yArn.Failure? then
+      false
+    else
+      AwsKmsMrkMatchForDecrypt.AwsKmsMrkMatchForDecrypt(AwsKmsArnIdentifier(xArn.value), AwsKmsArnIdentifier(yArn.value))
+  }
+
+  predicate HasKeyId(kmsConfiguration: Types.KMSConfiguration)
+  {
+    kmsConfiguration.kmsKeyArn? || kmsConfiguration.kmsMRKeyArn?
   }
 
   function GetKeyId(kmsConfiguration: Types.KMSConfiguration) : KMS.KeyIdType
+    requires HasKeyId(kmsConfiguration)
   {
     match kmsConfiguration
     case kmsKeyArn(arn) => arn
@@ -43,14 +100,16 @@ module {:options "/functionSyntax:4" } KMSKeystoreOperations {
     kmsClient: KMS.IKMSClient
   )
     returns (res: Result<KMS.GenerateDataKeyWithoutPlaintextResponse, Types.Error>)
-    requires AttemptKmsOperation?(kmsConfiguration, encryptionContext)
     requires kmsClient.ValidState()
+    requires HasKeyId(kmsConfiguration) && KmsArn.ValidKmsArn?(GetKeyId(kmsConfiguration))
+    requires AttemptKmsOperation?(kmsConfiguration, encryptionContext)
     modifies kmsClient.Modifies
     ensures kmsClient.ValidState()
     ensures
       && |kmsClient.History.GenerateDataKeyWithoutPlaintext| == |old(kmsClient.History.GenerateDataKeyWithoutPlaintext)| + 1
+      && var kmsKeyArn := GetKeyId(kmsConfiguration);
       && KMS.GenerateDataKeyWithoutPlaintextRequest(
-           KeyId := GetKeyId(kmsConfiguration),
+           KeyId := kmsKeyArn,
            EncryptionContext := Some(encryptionContext),
            KeySpec := None,
            NumberOfBytes := Some(32),
@@ -68,8 +127,9 @@ module {:options "/functionSyntax:4" } KMSKeystoreOperations {
               && kmsOperationOutput.Success?
               && kmsOperationOutput.value == res.value
   {
+    var kmsKeyArn := GetKeyId(kmsConfiguration);
     var generatorRequest := KMS.GenerateDataKeyWithoutPlaintextRequest(
-      KeyId := GetKeyId(kmsConfiguration),
+      KeyId := kmsKeyArn,
       EncryptionContext := Some(encryptionContext),
       KeySpec := None,
       NumberOfBytes := Some(32),
@@ -115,17 +175,19 @@ module {:options "/functionSyntax:4" } KMSKeystoreOperations {
            && destinationEncryptionContext == Structure.ActiveBranchKeyEncryptionContext(sourceEncryptionContext)
          )
     requires AttemptKmsOperation?(kmsConfiguration, destinationEncryptionContext)
+    requires HasKeyId(kmsConfiguration) && KmsArn.ValidKmsArn?(GetKeyId(kmsConfiguration))
     requires kmsClient.ValidState()
     modifies kmsClient.Modifies
     ensures kmsClient.ValidState()
 
     ensures
       && |kmsClient.History.ReEncrypt| == |old(kmsClient.History.ReEncrypt)| + 1
+      && var kmsKeyArn := GetKeyId(kmsConfiguration);
       && KMS.ReEncryptRequest(
            CiphertextBlob := ciphertext,
            SourceEncryptionContext := Some(sourceEncryptionContext),
-           SourceKeyId := Some(GetKeyId(kmsConfiguration)),
-           DestinationKeyId := GetKeyId(kmsConfiguration),
+           SourceKeyId := Some(kmsKeyArn),
+           DestinationKeyId := kmsKeyArn,
            DestinationEncryptionContext := Some(destinationEncryptionContext),
            SourceEncryptionAlgorithm := None,
            DestinationEncryptionAlgorithm := None,
@@ -136,21 +198,23 @@ module {:options "/functionSyntax:4" } KMSKeystoreOperations {
       && old(kmsClient.History.GenerateDataKeyWithoutPlaintext) == kmsClient.History.GenerateDataKeyWithoutPlaintext
 
     ensures res.Success? ==>
+              && var kmsKeyArn := GetKeyId(kmsConfiguration);
               && res.value.CiphertextBlob.Some?
               && res.value.SourceKeyId.Some?
               && res.value.KeyId.Some?
-              && res.value.SourceKeyId.value == GetKeyId(kmsConfiguration)
-              && res.value.KeyId.value == GetKeyId(kmsConfiguration)
+              && res.value.SourceKeyId.value == kmsKeyArn
+              && res.value.KeyId.value == kmsKeyArn
               && KMS.IsValid_CiphertextType(res.value.CiphertextBlob.value)
               && var kmsOperationOutput := Seq.Last(kmsClient.History.ReEncrypt).output;
               && kmsOperationOutput.Success?
               && kmsOperationOutput.value == res.value
   {
+    var kmsKeyArn := GetKeyId(kmsConfiguration);
     var reEncryptRequest := KMS.ReEncryptRequest(
       CiphertextBlob := ciphertext,
       SourceEncryptionContext := Some(sourceEncryptionContext),
-      SourceKeyId := Some(GetKeyId(kmsConfiguration)),
-      DestinationKeyId := GetKeyId(kmsConfiguration),
+      SourceKeyId := Some(kmsKeyArn),
+      DestinationKeyId := kmsKeyArn,
       DestinationEncryptionContext := Some(destinationEncryptionContext),
       SourceEncryptionAlgorithm := None,
       DestinationEncryptionAlgorithm := None,
@@ -164,10 +228,10 @@ module {:options "/functionSyntax:4" } KMSKeystoreOperations {
     :- Need(
       && reEncryptResponse.SourceKeyId.Some?
       && reEncryptResponse.KeyId.Some?
-      && reEncryptResponse.SourceKeyId.value == GetKeyId(kmsConfiguration)
-      && reEncryptResponse.KeyId.value == GetKeyId(kmsConfiguration),
+      && reEncryptResponse.SourceKeyId.value == kmsKeyArn
+      && reEncryptResponse.KeyId.value == kmsKeyArn,
       Types.KeyStoreException(
-        message := "Invalid response from KMS GenerateDataKey:: Invalid Key Id")
+        message := "Invalid response from KMS ReEncrypt:: Invalid Key Id")
     );
 
     :- Need(
@@ -188,8 +252,9 @@ module {:options "/functionSyntax:4" } KMSKeystoreOperations {
     kmsClient: KMS.IKMSClient
   )
     returns (output: Result<KMS.DecryptResponse, Types.Error>)
-    requires AttemptKmsOperation?(kmsConfiguration, encryptionContext)
+    requires KmsArn.ValidKmsArn?(encryptionContext[Structure.KMS_FIELD])
     requires item == Structure.ToAttributeMap(encryptionContext, item[Structure.BRANCH_KEY_FIELD].B)
+    requires AttemptKmsOperation?(kmsConfiguration, encryptionContext)
 
     requires kmsClient.ValidState()
     modifies kmsClient.Modifies
@@ -197,13 +262,14 @@ module {:options "/functionSyntax:4" } KMSKeystoreOperations {
 
     ensures
       && |kmsClient.History.Decrypt| == |old(kmsClient.History.Decrypt)| + 1
+      && var kmsKeyArn := GetArn(kmsConfiguration, encryptionContext[Structure.KMS_FIELD]);
       && KMS.DecryptRequest(
-           CiphertextBlob := item[Structure.BRANCH_KEY_FIELD].B,
-           EncryptionContext := Some(encryptionContext),
-           GrantTokens := Some(grantTokens),
-           KeyId := Some(GetKeyId(kmsConfiguration)),
-           EncryptionAlgorithm := None
-         )
+        CiphertextBlob := item[Structure.BRANCH_KEY_FIELD].B,
+        EncryptionContext := Some(encryptionContext),
+        GrantTokens := Some(grantTokens),
+        KeyId := Some(kmsKeyArn),
+        EncryptionAlgorithm := None
+      )
          == Seq.Last(kmsClient.History.Decrypt).input
     ensures output.Success?
             ==>
@@ -212,13 +278,13 @@ module {:options "/functionSyntax:4" } KMSKeystoreOperations {
               && output.value.Plaintext.Some?
               && 32 == |output.value.Plaintext.value|
   {
-
+    var kmsKeyArn := GetArn(kmsConfiguration, encryptionContext[Structure.KMS_FIELD]);
     var maybeDecryptResponse := kmsClient.Decrypt(
       KMS.DecryptRequest(
         CiphertextBlob := item[Structure.BRANCH_KEY_FIELD].B,
         EncryptionContext := Some(encryptionContext),
         GrantTokens := Some(grantTokens),
-        KeyId := Some(GetKeyId(kmsConfiguration)),
+        KeyId := Some(kmsKeyArn),
         EncryptionAlgorithm := None
       )
     );
