AwsCryptographicMaterialProviders/dafny/AwsCryptographyKeyStore/src/ErrorMessages.dfy
@@ -1,0 +1,39 @@
+// Copyright Amazon.com Inc. or its affiliates. All Rights Reserved.
+// SPDX-License-Identifier: Apache-2.0
+
+module {:options "/functionSyntax:4" } KeyStoreErrorMessages {
+  const KMS_CONFIG_KMS_ARN_INVALID :=
+    "KMSConfiguration's KMS Key ARN is invalid."
+
+  const CUSTOM_BRANCH_KEY_ID_NEED_EC :=
+    "Custom branch key identifier requires custom encryption context."
+
+  const GET_KEY_ARN_DISAGREEMENT :=
+    "Branch key's KMS Key ARN read from Dynamodb does not match Key Store's configured KMS Key ARN."
+
+  const DISCOVERY_CREATE_KEY_NOT_SUPPORTED :=
+    "Key Store's kmsConfiguration MUST BE kmsKeyArn or kmsMRKeyArn to Create Branch Keys."
+
+  const DISCOVERY_VERSION_KEY_NOT_SUPPORTED :=
+    "Key Store's kmsConfiguration MUST BE kmsKeyArn or kmsMRKeyArn to Version Branch Keys."
+
+  const UTF8_ENCODING_ENCRYPTION_CONTEXT_ERROR :=
+    "Unable to UTF8 Encode element of Encryption Context."
+
+  // Leaving this here in case we decide we want a different error message
+  const VERSION_KEY_KMS_KEY_ARN_DISAGREEMENT := GET_KEY_ARN_DISAGREEMENT
+
+  // Message assumes KMS resourceTypes are only [ alias, key ]
+  const ALIAS_NOT_ALLOWED :=
+    "Key Store encountered a KMS Alias ARN instead of a KMS Key ARN, which is not allowed."
+
+  const NO_CORRESPONDING_BRANCH_KEY :=
+    "No item found for corresponding branch key identifier."
+
+  const BRANCH_KEY_ID_NEEDED :=
+    "Empty string not supported for branch key identifier."
+
+  // If the Item/Record contains an invalid KMS ARN
+  const RETRIEVED_KEYSTORE_ITEM_INVALID_KMS_ARN :=
+    "The `kms-arn` field for the requested branch key identifier is corrupted."
+}
